src/goose_lang/examples/goose_semantics.v
@@ -407,8 +407,8 @@ Definition testBreakFromLoopWithContinue: val :=
       else Continue));;
     (![uint64T] "i" = #1).
 
-Definition failing_testBreakFromLoopNoContinue: val :=
-  rec: "failing_testBreakFromLoopNoContinue" <> :=
+Definition testBreakFromLoopNoContinue: val :=
+  rec: "testBreakFromLoopNoContinue" <> :=
     let: "i" := ref_to uint64T #0 in
     Skip;;
     (for: (λ: <>, ![uint64T] "i" < #3); (λ: <>, Skip) := λ: <>,
@@ -416,8 +416,44 @@ Definition failing_testBreakFromLoopNoContinue: val :=
       then
         "i" <-[uint64T] ![uint64T] "i" + #1;;
         Break
-      else "i" <-[uint64T] ![uint64T] "i" + #2);;
+      else "i" <-[uint64T] ![uint64T] "i" + #2));;
+    (![uint64T] "i" = #1).
+
+Definition failing_testBreakFromLoopNoContinueDouble: val :=
+  rec: "failing_testBreakFromLoopNoContinueDouble" <> :=
+    let: "i" := ref_to uint64T #0 in
+    Skip;;
+    (for: (λ: <>, ![uint64T] "i" < #3); (λ: <>, Skip) := λ: <>,
+      (if: (![uint64T] "i" = #1)
+      then
+        "i" <-[uint64T] ![uint64T] "i" + #1;;
+        Break
+      else
+        "i" <-[uint64T] ![uint64T] "i" + #2;;
+        "i" <-[uint64T] ![uint64T] "i" + #2));;
+    (![uint64T] "i" = #4).
+
+Definition testBreakFromLoopForOnly: val :=
+  rec: "testBreakFromLoopForOnly" <> :=
+    let: "i" := ref_to uint64T #0 in
+    Skip;;
+    (for: (λ: <>, ![uint64T] "i" < #3); (λ: <>, Skip) := λ: <>,
+      "i" <-[uint64T] ![uint64T] "i" + #2;;
       Continue);;
+    (![uint64T] "i" = #4).
+
+Definition testBreakFromLoopAssignAndContinue: val :=
+  rec: "testBreakFromLoopAssignAndContinue" <> :=
+    let: "i" := ref_to uint64T #0 in
+    Skip;;
+    (for: (λ: <>, ![uint64T] "i" < #3); (λ: <>, Skip) := λ: <>,
+      (if: #true
+      then
+        "i" <-[uint64T] ![uint64T] "i" + #1;;
+        Break
+      else
+        "i" <-[uint64T] ![uint64T] "i" + #2;;
+        Continue));;
     (![uint64T] "i" = #1).
 
 Definition testNestedLoops: val :=
@@ -441,6 +477,20 @@ Definition testNestedLoops: val :=
 
 Definition testNestedGoStyleLoops: val :=
   rec: "testNestedGoStyleLoops" <> :=
+    let: "ok" := ref_to boolT #false in
+    let: "i" := ref_to uint64T #0 in
+    (for: (λ: <>, ![uint64T] "i" < #10); (λ: <>, "i" <-[uint64T] ![uint64T] "i" + #1) := λ: <>,
+      let: "j" := ref_to uint64T #0 in
+      (for: (λ: <>, ![uint64T] "j" < ![uint64T] "i"); (λ: <>, "j" <-[uint64T] ![uint64T] "j" + #1) := λ: <>,
+        (if: #true
+        then Break
+        else Continue));;
+      "ok" <-[boolT] (![uint64T] "i" = #9);;
+      Continue);;
+    ![boolT] "ok".
+
+Definition testNestedGoStyleLoopsNoComparison: val :=
+  rec: "testNestedGoStyleLoopsNoComparison" <> :=
     let: "ok" := ref_to boolT #false in
     let: "i" := ref_to uint64T #0 in
     (for: (λ: <>, ![uint64T] "i" < #10); (λ: <>, "i" <-[uint64T] ![uint64T] "i" + #1) := λ: <>,
