external/Goose/github_com/mit_pdos/goose_nfsd/buftxn.v
@@ -7,20 +7,45 @@ From Goose Require github_com.mit_pdos.goose_nfsd.buf.
 From Goose Require github_com.mit_pdos.goose_nfsd.txn.
 From Goose Require github_com.mit_pdos.goose_nfsd.util.
 
+(* buftxn manages "buffer"-based transactions
+
+   The caller uses this interface by creating a BufTxn, reading/writing within
+   the transaction, and finally committing the buffered transaction.
+
+   Note that while the API has reads and writes, these are not the usual database
+   read/write transactions. Only writes are made atomic and visible atomically;
+   reads are cached on first read. Thus to use this library the file
+   system in practice locks (sub-block) objects before running a transaction.
+   This is necessary so that loaded objects are read from a consistent view.
+
+   Transactions support asynchronous durability by setting wait=false in
+   CommitWait. An asynchronous transaction is made visible atomically to other
+   threads, including across crashes, but if the system crashes a committed
+   asynchronous transaction can be lost. To guarantee that a particular
+   transaction is durable, call ( *Buftxn) Flush (which flushes all transactions).
+
+   Objects have sizes. Implicit in the code is that there is a static "schema"
+   that determines the disk layout: each block has objects of a particular size,
+   and all sizes used fit an integer number of objects in a block. This schema
+   guarantees that objects never overlap, as long as operations involving an
+   addr.Addr use the correct size for that block number.
+   The file system realizes this schema fairly simply,
+   since statically-allocated blocks are used for bitmap allocators (
+   objects are bits), inodes *)
+
 Module BufTxn.
   Definition S := struct.decl [
     "txn" :: struct.ptrT txn.Txn.S;
-    "bufs" :: struct.ptrT buf.BufMap.S;
-    "Id" :: uint64T
+    "bufs" :: struct.ptrT buf.BufMap.S
   ].
 End BufTxn.
 
+(* Start a local transaction with no writes from a global Txn manager. *)
 Definition Begin: val :=
   rec: "Begin" "txn" :=
     let: "trans" := struct.new BufTxn.S [
       "txn" ::= "txn";
-      "bufs" ::= buf.MkBufMap #();
-      "Id" ::= txn.Txn__GetTransId "txn"
+      "bufs" ::= buf.MkBufMap #()
     ] in
     util.DPrintf #1 (#(str"Begin: %v
     ")) #();;
@@ -36,7 +61,7 @@ Definition BufTxn__ReadBuf: val :=
       buf.BufMap__Lookup (struct.loadF BufTxn.S "bufs" "buftxn") "addr"
     else "b").
 
-(* Caller overwrites addr without reading it *)
+(* OverWrite writes an object to addr *)
 Definition BufTxn__OverWrite: val :=
   rec: "BufTxn__OverWrite" "buftxn" "addr" "sz" "data" :=
     let: "b" := ref_to (refT (struct.t buf.Buf.S)) (buf.BufMap__Lookup (struct.loadF BufTxn.S "bufs" "buftxn") "addr") in
@@ -54,24 +79,40 @@ Definition BufTxn__OverWrite: val :=
       struct.storeF buf.Buf.S "Data" (![refT (struct.t buf.Buf.S)] "b") "data";;
       buf.Buf__SetDirty (![refT (struct.t buf.Buf.S)] "b")).
 
+(* NDirty reports an upper bound on the size of this transaction when committed.
+
+   The caller cannot rely on any particular properties of this function for
+   safety. *)
 Definition BufTxn__NDirty: val :=
   rec: "BufTxn__NDirty" "buftxn" :=
     buf.BufMap__Ndirty (struct.loadF BufTxn.S "bufs" "buftxn").
 
+(* LogSz returns 511 *)
 Definition BufTxn__LogSz: val :=
   rec: "BufTxn__LogSz" "buftxn" :=
     txn.Txn__LogSz (struct.loadF BufTxn.S "txn" "buftxn").
 
+(* LogSzBytes returns 511*4096 *)
 Definition BufTxn__LogSzBytes: val :=
   rec: "BufTxn__LogSzBytes" "buftxn" :=
     txn.Txn__LogSz (struct.loadF BufTxn.S "txn" "buftxn") * disk.BlockSize.
 
-(* Commit dirty bufs of this transaction *)
+(* CommitWait commits the writes in the transaction to disk.
+
+   If CommitWait returns false, the transaction failed and had no logical effect.
+   This can happen, for example, if the transaction is too big to fit in the
+   on-disk journal.
+
+   wait=true is a synchronous commit, which is durable as soon as CommitWait
+   returns.
+
+   wait=false is an asynchronous commit, which can be made durable later with
+   Flush. *)
 Definition BufTxn__CommitWait: val :=
   rec: "BufTxn__CommitWait" "buftxn" "wait" :=
-    util.DPrintf #1 (#(str"Commit %d w %v
+    util.DPrintf #1 (#(str"Commit %p w %v
     ")) #();;
-    let: "ok" := txn.Txn__CommitWait (struct.loadF BufTxn.S "txn" "buftxn") (buf.BufMap__DirtyBufs (struct.loadF BufTxn.S "bufs" "buftxn")) "wait" (struct.loadF BufTxn.S "Id" "buftxn") in
+    let: "ok" := txn.Txn__CommitWait (struct.loadF BufTxn.S "txn" "buftxn") (buf.BufMap__DirtyBufs (struct.loadF BufTxn.S "bufs" "buftxn")) "wait" in
     "ok".
 
 Definition BufTxn__Flush: val :=
