src/program_proof/kvs/specs.v
@@ -6,7 +6,7 @@ From Perennial.Helpers Require Import Transitions.
 From Perennial.program_proof Require Import proof_prelude.
 
 From Goose.github_com.mit_pdos.goose_nfsd Require Import kvs.
-From Perennial.program_proof Require Import txn.specs buftxn.specs.
+From Perennial.program_proof Require Import txn.txn_proof buftxn.buftxn_proof.
 From Perennial.program_proof Require Import proof_prelude.
 From Perennial.program_proof Require Import disk_lib.
 From Perennial.Helpers Require Import NamedProps Map List.
